DPLL/z3_files/phi-2n-1-smaller-than-0-base.py
@@ -1,8 +1,0 @@
-from sys import path
-path.insert(0,"/ubc/cs/home/y/yanpeng/project/ACL2/smtlink/z3_interface")
-from ACL2_translator import to_smt, Q
-s = to_smt()
-V0=s.isReal("V0")
-hypothesis=False
-conclusion=True
-s.prove(hypothesis, conclusion)
