smtlink/z3_files/smtlink_TTZPY.py
@@ -1,8 +1,0 @@
-from sys import path
-path.insert(0,"/ubc/cs/home/y/yanpeng/project/ACL2/smtlink/z3_interface")
-from ACL22SMT import to_smt, Q
-s = to_smt()
-X=s.isReal("X")
-hypothesis=True
-conclusion=s.equal(s.plus(X,X),s.times(1,(lambda var0:s.times(4,s.times(s.Qx(1,2),var0)))(X)))
-s.prove(hypothesis, conclusion)
