smtlink/SMT-z3.lisp
@@ -44,7 +44,7 @@
 )
 
 ;; my-prove-SMT-formula
-(defun my-prove-SMT-formula (term)
+(defun my-prove-SMT-formula (term uninterpreted)
   "my-prove-SMT-formula: check if term is a valid SMT formula"
   (let ((decl-list (cadr (cadr term)))
 	(hypo-list (caddr (cadr term)))
@@ -52,14 +52,26 @@
     (SMT-formula '()
 		 decl-list
 		 hypo-list
-		 concl-list)))
+		 concl-list
+     uninterpreted)))
+
+;; create-uninterpreted-formula
+(defun create-uninterpreted-formula (uninterpreted)
+  (if (endp uninterpreted)
+      nil
+    (cons (list (caar uninterpreted)
+                (caar uninterpreted)
+                (caddar uninterpreted))
+          (create-uninterpreted-formula (cdr uninterpreted)))))
 
 ;; my-prove-write-file
-(defun my-prove-write-file (term fdir smt-cnf state)
+(defun my-prove-write-file (term fdir smt-cnf uninterpreted state)
   "my-prove-write-file: write translated term into a file"
   (write-SMT-file fdir
 		  (translate-SMT-formula
-		   (my-prove-SMT-formula term))
+		   (my-prove-SMT-formula term
+                             (create-uninterpreted-formula uninterpreted))
+       uninterpreted)
 		  smt-cnf
 		  state))
 
@@ -161,9 +173,8 @@ new hypothesis in lambda expression"
 	       )))
 
 (defun augment-hypothesis (rewritten-term let-expr orig-param main-hints aux-thms state)
-  (prog2$ (cw "aux-thms: ~q0~%" aux-thms)
   (let ((res (augment-hypothesis-helper rewritten-term let-expr orig-param main-hints state)))
-    (add-aux res aux-thms))))
+    (add-aux res aux-thms)))
 
 ;;separate-type
 (defun separate-type (let-expr)
@@ -289,8 +300,45 @@ new hypothesis in lambda expression"
                  fname
                  ".py")))
 
+;; create-uninterpreted-item
+(defun create-uninterpreted-item (item)
+  (cons (car item)
+        (cons (head (cdr item))
+              (end (cdr item)))))
+
+;; uninterpreted-type-&-name: processing the list of uninterpreted functions
+;; produces an associate list. Key is the function name, value is a 2 element
+;; list. First element is a list of input argument type, second element is the
+;; return type.
+(defun uninterpreted-type-&-name (uninterpreted)
+  (if (endp uninterpreted)
+      nil
+    (cons (create-uninterpreted-item (car uninterpreted))
+          (uninterpreted-type-&-name (cdr uninterpreted))))
+  )
+
+;; create-proc-name
+;; given name "XXX", create name "s.XXX"
+;; User defined uninterpreted functions are assumed to be all in lower case
+(defun create-proc-name (name)
+  (concatenate 'string "s." (string-downcase (string name))))
+
+;; create-uninterpreted-oprt-item
+;; By default, using the same name in ACL2.
+(defun create-uninterpreted-oprt-item (item)
+  (list (car item)
+        (create-proc-name (car item))
+        (length (cadr item))))
+
+;; uninterpreted-operator
+(defun uninterpreted-operator (uninterpreted-assoc)
+  (if (endp uninterpreted-assoc)
+      nil
+    (cons (create-uninterpreted-oprt-item (car uninterpreted-assoc))
+          (uninterpreted-operator (cdr uninterpreted-assoc)))))
+
 ;; my-prove
-(defun my-prove (term fn-lst fn-level fname let-expr new-hypo let-hints hypo-hints main-hints smt-cnf state)
+(defun my-prove (term fn-lst fn-level uninterpreted fname let-expr new-hypo let-hints hypo-hints main-hints smt-cnf state)
   "my-prove: return the result of calling SMT procedure"
   (let ((file-dir (mk-fname fname smt-cnf))
 	(expand-dir (concatenate 'string
@@ -298,6 +346,9 @@ new hypothesis in lambda expression"
 				 "/"
 				 fname
 				 "\_expand.log")))
+    (let ((uninterpreted-func
+           (uninterpreted-operator
+            (uninterpreted-type-&-name uninterpreted))))
     (mv-let (hypo-translated state)
 	    (translate-hypo new-hypo state)
     (mv-let (let-expr-translated-with-type state)
@@ -318,7 +369,9 @@ new hypothesis in lambda expression"
 							    expanded-term-list
 							    file-dir
 							    smt-cnf
-							    state)))
+                  uninterpreted-func
+							    state)
+                       ))
 						(let ((type-theorem (create-type-theorem (cadr term)
 											 let-expr-translated
 											 let-type
@@ -342,4 +395,4 @@ new hypothesis in lambda expression"
 											 state)))
 						  (if (car (SMT-interpreter file-dir smt-cnf))
 						      (mv t aug-theorem type-theorem hypo-theorem fn-type-theorem state)
-						      (mv nil aug-theorem type-theorem hypo-theorem fn-type-theorem state))))))))))))))
+						      (mv nil aug-theorem type-theorem hypo-theorem fn-type-theorem state)))))))))))))))
